verify/Extraction.v
@@ -1,9 +1,10 @@
 (** * Extraction to OCaml *)
 
 From Coq Require Extraction.
+From Coq Require Import Lists.List. Import ListNotations.
 Require Import ExtrOcamlBasic.
 Require Import ExtrOcamlIntConv.
-From BusyCoq Require Export TranslatedCyclers.
+From BusyCoq Require Export BackwardsReasoning.
 
 Inductive state := A | B | C | D | E.
 Inductive sym := S0 | S1.
@@ -40,12 +41,28 @@ Module Ctx <: Ctx.
   Proof.
     intros [] []; constructor; (reflexivity || discriminate).
   Qed.
+
+  Definition all_qs := [A; B; C; D; E].
+
+  Lemma all_qs_spec : forall a, In a all_qs.
+  Proof.
+    destruct a; repeat ((left; reflexivity) || right).
+  Qed.
+
+  Definition all_syms := [S0; S1].
+
+  Lemma all_syms_spec : forall a, In a all_syms.
+  Proof.
+    destruct a; repeat ((left; reflexivity) || right).
+  Qed.
 End Ctx.
 
 Module ECyclers := Cyclers Ctx.
 Module ETranslatedCyclers := TranslatedCyclers Ctx.
+Module EBackwardsReasoning := BackwardsReasoning Ctx.
 
 Extraction Language OCaml.
 Extraction "extraction.ml" nat_of_int
   ECyclers.verify_cycler
-  ETranslatedCyclers.verify_tcycler.
+  ETranslatedCyclers.verify_tcycler
+  EBackwardsReasoning.verify_backwards.
