verify/BackwardsReasoning.v
@@ -1,0 +1,197 @@
+(** * Backwards Reasoning *)
+
+From Coq Require Import Bool.Bool.
+From Coq Require Import Arith.Arith.
+From Coq Require Import Lia.
+From Coq Require Import Lists.Streams.
+From Coq Require Import Lists.List. Import ListNotations.
+From BusyCoq Require Export TranslatedCyclers.
+Set Default Goal Selector "!".
+
+Module BackwardsReasoning (Ctx : Ctx).
+  Module TranslatedCyclers := TranslatedCyclers Ctx. Export TranslatedCyclers.
+
+Definition all_qs := list_prod all_qs all_syms.
+
+Lemma all_qs_spec : forall a, In a all_qs.
+Proof. introv. destruct a. apply in_prod; auto. Qed.
+
+Local Hint Resolve all_qs_spec : auto.
+
+Fixpoint side_matches (xs : side) (ys : list Sym) : Prop :=
+  match xs, ys with
+  | _, [] => True
+  | (Cons x xs), y :: ys => x = y /\ side_matches xs ys
+  end.
+
+Lemma side_matches_nil : forall xs, side_matches xs [].
+Proof. destruct xs. split. Qed.
+
+Lemma side_matches_cons : forall xs ys,
+  side_matches (Streams.tl xs) ys ->
+  side_matches xs (Streams.hd xs :: ys).
+Proof.
+  introv H. destruct xs. simpl in *. intuition.
+Qed.
+
+Local Hint Resolve side_matches_nil : core.
+Local Hint Resolve side_matches_cons : core.
+
+Definition stencil : Type := Q * ctape.
+
+Definition matches (t : Q * tape) (t' : stencil) : Prop :=
+  match t, t' with
+  | q;; l {{s}} r, q';; l' {{s'}} r' =>
+    q = q' /\ s = s' /\ side_matches l l' /\ side_matches r r'
+  end.
+
+Definition find_transitions (tm : TM) (f : option (Sym * dir * Q) -> bool)
+    : list (Q * Sym) :=
+  filter (fun a => f (tm a)) all_qs.
+
+Lemma find_transitions_In : forall tm f q s,
+  f (tm (q, s)) = true <->
+  In (q, s) (find_transitions tm f).
+Proof.
+  introv.
+  unfold find_transitions.
+  rewrite filter_In.
+  intuition.
+Qed.
+
+Definition halting_transitions (tm : TM) :=
+  find_transitions tm (fun cmd =>
+    match cmd with
+    | Some _ => false
+    | None => true
+    end).
+
+Definition haltings (tm : TM) : list stencil :=
+  map (fun '(q, s) => q;; [] {{s}} []) (halting_transitions tm).
+
+Lemma haltings_spec : forall tm c,
+  halting tm c -> Exists (matches c) (haltings tm).
+Proof.
+  introv H. destruct c as [q [[l s] r]].
+  unfold halting in H.
+  assert (Hfound : In (q, s) (halting_transitions tm)).
+  { unfold halting_transitions.
+    rewrite <- find_transitions_In.
+    rewrite H. reflexivity. }
+  eapply in_map in Hfound.
+  rewrite Exists_exists.
+  eexists. split.
+  - eassumption.
+  - repeat split; auto.
+Qed.
+
+Definition symbol_ok (t : ctape) (s' : Sym) (d : dir) :=
+  match d, t with
+  | L, _ {{_}} []       => true
+  | L, _ {{_}} (s :: _) => eqb_sym s s'
+  | R,       [] {{_}} _ => true
+  | R, (s :: _) {{_}} _ => eqb_sym s s'
+  end.
+
+(* If we took the [(q, s)] transition and ended up at [st], how did the
+   tape look before? *)
+Definition rewind (tm : TM) (st : stencil) (q : Q) (s : Sym) : option stencil :=
+  let '(qfin, tfin) := st in
+  match tm (q, s) with
+  | None => None
+  | Some (s', d, q') =>
+    if eqb_q qfin q' && symbol_ok tfin s' d then
+      let '(l, _, r) :=
+        match d with
+        | L => right tfin
+        | R => left tfin
+        end
+      in
+      Some (q;; l {{s}} r)
+    else
+      None
+  end.
+
+Lemma rewind_spec : forall tm q l s r c' st,
+  q;; l {{s}} r -[ tm ]-> c' ->
+  matches c' st ->
+  exists st0, rewind tm st q s = Some st0 /\ matches (q;; l {{s}} r) st0.
+Proof.
+  introv Hstep Hmatch.
+  destruct c' as [q' [[l' s'] r']].
+  destruct st as [q'' [[stl s''] str]].
+  destruct Hmatch as [Eq [Es [Hl Hr]]]. subst q'' s''.
+  inverts Hstep as Htm;
+    unfold rewind;
+    rewrite Htm, eqb_q_refl;
+    lazymatch goal with
+    | H: side_matches (?side << ?s) ?st |- _ =>
+      destruct st; [clear H | inverts H]
+    end; simpl;
+    eexists; try rewrite eqb_sym_refl;
+    repeat split; auto.
+Qed.
+
+Fixpoint has_contra (tm : TM) (n : nat) (st : stencil) :=
+  match n with
+  | O => false
+  | S n =>
+    forallb (fun '(q, s) =>
+      match rewind tm st q s with
+      | Some st' => has_contra tm n st'
+      | None => true
+      end)
+      all_qs
+  end.
+
+Theorem has_contra_spec : forall tm n c c' st,
+  c -[ tm ]->> n / c' ->
+  matches c' st ->
+  has_contra tm n st = true ->
+  False.
+Proof.
+  induction n; introv Hrun Hmatches Hcontra.
+  - discriminate.
+  - apply multistep_last in Hrun.
+    destruct Hrun as [c'' [Hrun Hstep]].
+    simpl in Hcontra. rewrite forallb_forall in Hcontra.
+    destruct c'' as [q [[l s] r]].
+    specialize (Hcontra (q, s) (all_qs_spec _)).
+    simpl in Hcontra.
+    apply rewind_spec with (st := st) in Hstep; try assumption.
+    destruct Hstep as [st' [Erewind Hmatches']].
+    rewrite Erewind in Hcontra.
+    eauto.
+Qed.
+
+Definition verify_backwards (tm : TM) (n : nat) : bool :=
+  match cmultistep tm n starting with
+  | Some _ => forallb (has_contra tm n) (haltings tm)
+  | None => false
+  end.
+
+Theorem verify_backwards_correct : forall tm n,
+  verify_backwards tm n = true ->
+  ~ halts tm c0.
+Proof.
+  introv H Hhalts. unfold verify_backwards in H.
+  destruct (cmultistep tm n starting) eqn:E; try discriminate.
+  apply cmultistep_some in E.
+  destruct Hhalts as [m Hhalts].
+  assert (Hle : n <= m)
+    by eauto using within_halt.
+
+  destruct Hhalts as [ch [Hhaltrun Hhalting]].
+  replace m with ((m - n) + n) in Hhaltrun by lia.
+  apply rewind_split in Hhaltrun.
+  destruct Hhaltrun as [c1 [Hrun1 Hrun2]].
+
+  apply haltings_spec in Hhalting.
+  rewrite Exists_exists in Hhalting.
+  destruct Hhalting as [st [Hin Hmatches]].
+
+  rewrite forallb_forall in H. apply H in Hin.
+  eapply has_contra_spec; eassumption.
+Qed.
+
+End BackwardsReasoning.
