verify/TM.v
@@ -1,6 +1,7 @@
 (** * TM: Definition of Turing Machines *)
 
-From Coq Require Export Lists.Streams.
+From Coq Require Import Lists.List. Import ListNotations.
+From Coq Require Import Lists.Streams.
 From Coq Require Import PeanoNat.
 From Coq Require Import Lia.
 From BusyCoq Require Export Helper.
@@ -25,10 +26,25 @@ Module Type Ctx.
   Parameter eqb_q_spec : forall a b, reflect (a = b) (eqb_q a b).
   Parameter eqb_sym : Sym -> Sym -> bool.
   Parameter eqb_sym_spec : forall a b, reflect (a = b) (eqb_sym a b).
+
+  (** It is also useful, in some situations, to be able to enumerate
+      all the symbols and states. *)
+  Parameter all_qs : list Q.
+  Parameter all_qs_spec : forall a, In a all_qs.
+  Parameter all_syms : list Sym.
+  Parameter all_syms_spec : forall a, In a all_syms.
 End Ctx.
 
 Module TM (Ctx : Ctx).
   Export Ctx.
+
+Lemma eqb_q_refl : forall q, eqb_q q q = true.
+Proof. introv. destruct (eqb_q_spec q q); congruence. Qed.
+
+Lemma eqb_sym_refl : forall s, eqb_sym s s = true.
+Proof. introv. destruct (eqb_sym_spec s s); congruence. Qed.
+
+#[export] Hint Resolve all_qs_spec all_syms_spec : core.
 
 (** A Turing machine is a function mapping each [(state, symbol)] pair
     to one of
@@ -40,10 +56,12 @@ Module TM (Ctx : Ctx).
 *)
 Definition TM : Type := Q * Sym -> option (Sym * dir * Q).
 
+Notation side := (Stream Sym).
+
 (** The state of the tape is represented abstractly as a tuple [(l, s, r)],
     where [v] is the symbol under the head, while [l] and [r] are infinite
     streams of symbols on the left and right side of the head, respectively. *)
-Definition tape : Type := Stream Sym * Sym * Stream Sym.
+Definition tape : Type := side * Sym * side.
 
 (** We define a notation for tapes, evocative of a turing machine's head
     hovering over a particular symbol. **)
@@ -99,6 +117,8 @@ Inductive multistep (tm : TM) : nat -> Q * tape -> Q * tape -> Prop :=
 
   where "c -[ tm ]->> n / c'" := (multistep tm n c c').
 
+#[export] Hint Constructors multistep : core.
+
 (** Executing an unspecified number of steps (the "eventually
     reaches" relation): *)
 Reserved Notation "c -[ tm ]->* c'" (at level 40).
@@ -111,6 +131,8 @@ Inductive evstep (tm : TM) : Q * tape -> Q * tape -> Prop :=
     c  -[ tm ]->* c''
 
   where "c -[ tm ]->* c'" := (evstep tm c c').
+
+#[export] Hint Constructors evstep : core.
 
 (** Executing an unspecified, but non-zero number of steps: *)
 Reserved Notation "c -[ tm ]->+ c'" (at level 40).
@@ -125,6 +147,8 @@ Inductive progress (tm : TM) : Q * tape -> Q * tape -> Prop :=
     c  -[ tm ]->+ c''
 
   where "c -[ tm ]->+ c'" := (progress tm c c').
+
+#[export] Hint Constructors progress : core.
 
 (** A halting configuration is one for which [tm (q, s)] returns [None]. *)
 Definition halting (tm : TM) (c : Q * tape) : Prop :=
@@ -208,15 +232,24 @@ Proof.
     assumption.
 Qed.
 
+Lemma multistep_last :
+  forall tm n c c'',
+  c -[ tm ]->> S n / c'' ->
+  exists c', c -[ tm ]->> n / c' /\ c' -[ tm ]-> c''.
+Proof.
+  induction n; introv H; inverts H as H1 H2.
+  - inverts H2. eauto.
+  - apply IHn in H2. destruct H2 as [cmid [H2 H3]].
+    eauto.
+Qed.
+
 Lemma evstep_trans :
   forall tm c c' c'',
   c  -[ tm ]->* c'  ->
   c' -[ tm ]->* c'' ->
   c  -[ tm ]->* c''.
 Proof.
-  introv H1 H2. induction H1.
-  - apply H2.
-  - eauto using evstep_step.
+  introv H1 H2. induction H1; eauto.
 Qed.
 
 Lemma progress_trans :
@@ -225,7 +258,7 @@ Lemma progress_trans :
   c' -[ tm ]->+ c'' ->
   c  -[ tm ]->+ c''.
 Proof.
-  introv H1 H2. induction H1; eauto using progress_step.
+  introv H1 H2. induction H1; eauto.
 Qed.
 
 Lemma multistep_progress :
@@ -234,8 +267,8 @@ Lemma multistep_progress :
   c -[ tm ]->+ c'.
 Proof.
   induction n; introv H; inverts H as Hstep Hrest.
-  - inverts Hrest. apply progress_base. assumption.
-  - apply IHn in Hrest. eapply progress_step; eassumption.
+  - inverts Hrest. auto.
+  - eauto.
 Qed.
 
 Lemma progress_multistep :
@@ -245,9 +278,9 @@ Lemma progress_multistep :
   c -[ tm ]->> S n / c'.
 Proof.
   introv H. induction H.
-  - eauto using multistep_S, multistep_0.
+  - eauto.
   - destruct IHprogress as [n IH].
-    eauto using multistep_S.
+    eauto.
 Qed.
 
 Lemma without_counter :
@@ -255,9 +288,7 @@ Lemma without_counter :
   c -[ tm ]->> n / c' ->
   c -[ tm ]->* c'.
 Proof.
-  introv H. induction H.
-  - apply evstep_refl.
-  - eauto using evstep_step.
+  introv H. induction H; eauto.
 Qed.
 
 Lemma with_counter :
@@ -266,9 +297,9 @@ Lemma with_counter :
   exists n, c -[ tm ]->> n / c'.
 Proof.
   introv H. induction H.
-  - exists 0. apply multistep_0.
+  - eauto.
   - destruct IHevstep as [n IH].
-    eauto using multistep_S.
+    eauto.
 Qed.
 
 Lemma evstep_progress :
@@ -292,7 +323,7 @@ Lemma evstep_progress_trans :
 Proof.
   introv H1 H2. induction H1.
   - exact H2.
-  - eauto using progress_step.
+  - eauto.
 Qed.
 
 Lemma progress_evstep_trans :
@@ -304,9 +335,9 @@ Proof.
   introv H1 H2. induction H1.
   - apply with_counter in H2.
     destruct H2 as [[| n] H2].
-    + inverts H2. apply progress_base. assumption.
-    + apply multistep_progress in H2. eauto using progress_step.
-  - eauto using progress_step.
+    + inverts H2. auto.
+    + apply multistep_progress in H2. eauto.
+  - eauto.
 Qed.
 
 Lemma rewind_split:
@@ -316,15 +347,11 @@ Lemma rewind_split:
 Proof.
   intros tm n k.
   induction n; intros c c'' H.
-  - exists c. split.
-    + apply multistep_0.
-    + assumption.
+  - eauto.
   - inverts H as Hstep Hrest.
     apply IHn in Hrest. clear IHn.
     destruct Hrest as [cn [Hn Hk]].
-    exists cn. split.
-    + eapply multistep_S; eassumption.
-    + exact Hk.
+    eauto.
 Qed.
 
 Lemma halting_no_multistep:
@@ -354,6 +381,16 @@ Proof.
   eapply halting_no_multistep in Hhalting.
   - apply Hhalting. eassumption.
   - lia.
+Qed.
+
+Corollary within_halt : forall tm c c' k n,
+  halts_in tm c n ->
+  c -[ tm ]->> k / c' ->
+  k <= n.
+Proof.
+  introv Hhalts Hrun.
+  destruct (Nat.leb_spec k n); try assumption.
+  exfalso. eauto using exceeds_halt.
 Qed.
 
 Lemma preceeds_halt : forall tm c c' n k,
